opt_pipelines.v
@@ -128,6 +128,10 @@ Require Import FORVES2.optimizations.and_coinbase.
 Import Opt_and_coinbase.
 Require Import FORVES2.optimizations.balance_address.
 Import Opt_balance_address.
+Require Import FORVES2.optimizations.slt_x_x.
+Import Opt_slt_x_x.
+Require Import FORVES2.optimizations.sgt_x_x.
+Import Opt_sgt_x_x.
 
 
 Module OptPipelines.
@@ -195,6 +199,8 @@ Inductive available_optimization_step :=
 | OPT_and_ffff
 | OPT_and_coinbase
 | OPT_balance_address
+| OPT_slt_x_x
+| OPT_sgt_x_x
 .
 
 Definition list_opt_steps := list available_optimization_step.
@@ -263,6 +269,8 @@ match tag with
 | OPT_and_ffff => OpEntry optimize_and_ffff_sbinding optimize_and_ffff_sbinding_snd
 | OPT_and_coinbase => OpEntry optimize_and_coinbase_sbinding optimize_and_coinbase_sbinding_snd
 | OPT_balance_address => OpEntry optimize_balance_address_sbinding optimize_balance_address_sbinding_snd
+| OPT_slt_x_x => OpEntry optimize_slt_x_x_sbinding optimize_slt_x_x_sbinding_snd
+| OPT_sgt_x_x => OpEntry optimize_sgt_x_x_sbinding optimize_sgt_x_x_sbinding_snd
 end.
 
 Definition all_optimization_steps_gas : list_opt_steps := 
@@ -327,7 +335,9 @@ Definition all_optimization_steps_gas : list_opt_steps :=
    OPT_or_ffff;
    OPT_and_ffff;
    OPT_and_coinbase;
-   OPT_balance_address
+   OPT_balance_address;
+   OPT_slt_x_x;
+   OPT_sgt_x_x
 ].
 
 Definition all_optimization_steps_size := 
@@ -392,7 +402,9 @@ Definition all_optimization_steps_size :=
    OPT_or_ffff;
    OPT_and_ffff;
    OPT_and_coinbase;
-   OPT_balance_address
+   OPT_balance_address;
+   OPT_slt_x_x;
+   OPT_sgt_x_x
 ].
 
 End OptPipelines.
